

Q - Evaluate

$$\textcircled{1} \log_3 243$$

$$\textcircled{2} \log_{5\sqrt{2}} 2500$$

$$\textcircled{3} (1024)^{\log_2 m}$$

$$\textcircled{4} (729)^{\log_3 m}$$

$$\textcircled{5} \log_x \left(\frac{1}{x}\right)$$

$$\textcircled{6} \log 81 \div \log 27$$

$$\textcircled{2} \log_{5\sqrt{2}} (2500)$$

$$= \frac{\log 2500}{\log 5\sqrt{2}}$$

$$= \frac{\log (2500)}{\log (\sqrt{50})}$$

$$= \frac{\log (50)^2}{\log (50)^{1/2}}$$

$$= \frac{2 \times \log 50}{\frac{1}{2} \times \log 50}$$

$$= \frac{2}{\frac{1}{2}} = 2 \times 2 = 4$$

$$\begin{aligned} 5\sqrt{2} &= \sqrt{25 \times 2} \\ &= \sqrt{50} \end{aligned}$$

$$\textcircled{5} \log_x \left(\frac{1}{x}\right)$$

$$= \log_x (x)^{-1}$$

$$= (-1) \times \log_x x$$

$$= (-1) \times 1$$

$$= -1$$

$$\textcircled{4} (729)^{\log_3 m}$$

$$= (3^6)^{\log_3 m}$$

$$= (3)^{6 \times \log_3 m}$$

$$= (3)^{\log_3 (m)^6}$$

$$= (m)^6$$

$$\textcircled{1} \log_3 (243)$$

$$= \log_3 (3)^5$$

$$= 5 \times \log_3 3$$

$$= 5 \times 1$$

$$= 5$$

$$\textcircled{3} (1024)^{\log_2 m}$$

$$= (2^{10})^{\log_2 m}$$

$$= (2)^{10 \times \log_2 m}$$

$$= (2)^{\log_2 (m)^{10}}$$

$$= (m)^{10}$$

$$\textcircled{6} \log 81 \div \log 27$$

$$= \frac{\log 81}{\log 27}$$

$$= \frac{\log (3)^4}{\log (3)^3}$$

$$= \frac{4 \times \log 3}{3 \times \log 3}$$

$$= \frac{4}{3}$$

Q: → Prove that

$$\begin{aligned}\textcircled{1} \text{ L.H.S.} &= \log\left(\frac{9}{14}\right) - \log\left(\frac{15}{16}\right) + \log\left(\frac{35}{24}\right) \\&= \log\left(\frac{9}{14}\right) + \log\left(\frac{16}{15}\right) + \log\left(\frac{35}{24}\right) \\&= \log\left[\frac{9}{14} \times \frac{16}{15} \times \frac{35}{24}\right] \\&= \log[1] \\&= 0 \\&= \text{RHS}\end{aligned}$$

$$\begin{aligned}\textcircled{2} \text{ L.H.S.} &= \frac{1}{\log_{24} 12} + \frac{1}{\log_8 12} + \frac{1}{\log_9 12} \\&= \frac{1}{\frac{\log 12}{\log 24}} + \frac{1}{\frac{\log 12}{\log 8}} + \frac{1}{\frac{\log 12}{\log 9}} \\&= \frac{\log 24}{\log 12} + \frac{\log 8}{\log 12} + \frac{\log 9}{\log 12} \\&= \frac{\log 24 + \log 8 + \log 9}{\log 12} \\&= \frac{\log(24 \times 8 \times 9)}{\log 12} \\&= \frac{\log(1728)}{\log 12} = \frac{\log(12)^3}{\log 12} = \frac{3 \times \log 12}{\log 12} \\&= 3 \\&= \text{RHS}\end{aligned}$$

Q: → Prove that

$$\begin{aligned}
 \textcircled{3} \text{ L.H.S} &= \frac{1}{\log_2 64} + \frac{1}{\log_{\sqrt{2}} 64} + \frac{1}{\log_{2\sqrt{2}} 64} \\
 &= \frac{1}{\frac{\log 64}{\log 2}} + \frac{1}{\frac{\log 64}{\log \sqrt{2}}} + \frac{1}{\frac{\log 64}{\log 2\sqrt{2}}} \\
 &= \frac{\log 2}{\log 64} + \frac{\log \sqrt{2}}{\log 64} + \frac{\log 2\sqrt{2}}{\log 64} \\
 &= \frac{\log 2 + \log \sqrt{2} + \log 2\sqrt{2}}{\log 64} \\
 &= \frac{\log (2 \times \sqrt{2} \times 2\sqrt{2})}{\log 64} \\
 &= \frac{\log 8}{\log 64} = \frac{\log 8}{\log (8)^2} = \frac{\log 8}{2 \times \log 8} \\
 &= \frac{1}{2} = \text{RHS}
 \end{aligned}$$

$$\begin{aligned}
 \textcircled{4} \text{ L.H.S} &= \log (\sqrt{x^2+1} + x) + \log (\sqrt{x^2+1} - x) \\
 &= \log [(\sqrt{x^2+1} + x)(\sqrt{x^2+1} - x)] \\
 &\quad \left[ \begin{array}{l} (a+b)(a-b) = a^2 - b^2 \\ a = \sqrt{x^2+1} \quad b = x \end{array} \right] \\
 &= \log [(\sqrt{x^2+1})^2 - (x)^2] \\
 &= \log [x^2 + 1 - x^2] \\
 &= \log [1] \\
 &= 0 \\
 &= \text{RHS}
 \end{aligned}$$

Q: → Prove that

$$\begin{aligned} \textcircled{5} \quad \text{L.H.S} &= \log\left(\frac{32}{25}\right) + \log\left(\frac{64}{225}\right) + \log\left(\frac{25}{128}\right) + \log\left(\frac{450}{32}\right) \\ &= \log\left[\frac{\cancel{32}}{25} \times \frac{\cancel{64}}{225} \times \frac{25}{\cancel{128}} \times \frac{\cancel{25} \cdot 450}{\cancel{32}}\right] \\ &= \log[1] \\ &= 0 \\ &= \text{RHS.} \end{aligned}$$

Q: → Solve the following

$$\begin{aligned} \textcircled{1} \quad \log_x 243 &= 5 \\ \Rightarrow 243 &= (x)^5 \\ \Rightarrow (3)^5 &= (x)^5 \\ \Rightarrow 3 &= x \\ \Rightarrow x &= 3 \end{aligned}$$

$$\begin{aligned} \textcircled{2} \quad \log_{32} x &= \frac{2}{5} \\ \Rightarrow x &= (32)^{\frac{2}{5}} \\ \Rightarrow x &= (2^5)^{\frac{2}{5}} \\ \Rightarrow x &= (2)^{5 \times \frac{2}{5}} \\ \Rightarrow x &= (2)^2 \\ \Rightarrow x &= 4 \end{aligned}$$

$$\begin{aligned} \textcircled{3} \quad \frac{\log x \times \log 16}{\log 32} &= \log 256 \\ \therefore \log x &= \frac{\log 256 \times \log 32}{\log 16} \\ &= \frac{\log(2)^8 \times \log(2)^5}{\log(2)^4} \\ &= \frac{2 \times \log 2 \times 5 \times \log 2}{4 \times \log 2} \end{aligned}$$

$$= 2 \times 5 \times \log 2$$

$$\therefore \log x = 10 \times \log 2$$

$$\therefore \log x = \log(2)^{10}$$

By Taking Antilog

$$\therefore x = (2)^{10}$$

$$\therefore x = 1024$$



Q. → Solve the following

(4)  $\log_x 4 + \log_x 8 + \log_x 16 = 9$

$\therefore \log_x (4 \times 8 \times 16) = 9$

$\therefore \log_x (512) = 9$

$\therefore 512 = (x)^9$

$\therefore (2)^9 = (x)^9$

$\therefore 2 = x$

$\therefore x = 2$

(5)  $\log_2 (\log_3 (2x+1)) = 1$

$\left[ \begin{array}{l} p = \log_3 (2x+1) \\ \log_2 (p) = 1 \therefore p = (2)^1 \end{array} \right]$

$\therefore \log_3 (2x+1) = (2)^1$

$\therefore \log_3 (2x+1) = 2$

$\therefore (2x+1) = (3)^2$

$\therefore 2x+1 = 9$

$\therefore 2x = 9-1$

$\therefore 2x = 8$

$\therefore x = \frac{8}{2}$

$\therefore x = 4$

(6)  $\frac{1}{\log_8 x} + \frac{1}{\log_9 x} + \frac{1}{\log_{16} x} = 3$

$\therefore \frac{1}{\frac{\log x}{\log 8}} + \frac{1}{\frac{\log x}{\log 9}} + \frac{1}{\frac{\log x}{\log 16}} = 3$

$\therefore \frac{\log 8}{\log x} + \frac{\log 9}{\log x} + \frac{\log 16}{\log x} = 3$

$\therefore \frac{\log 8 + \log 9 + \log 16}{\log x} = 3$

$\therefore \frac{\log (8 \times 9 \times 16)}{\log x} = 3$

$\therefore \log (1152) = 3 \times \log x$

$\therefore \log (1152) = \log (x)^3$

By Taking Antilog

$1152 = x^3$

$\therefore x^3 = 1152$

$\therefore x^3 = (2)^3 \times (3)^2 \times (2)^4$

$= (2)^3 \times 9 \times (2)^3 \times 2$

$\therefore x^3 = (2)^3 \times (2)^3 \times 18$

$\therefore x = 2 \times 2 \times \sqrt[3]{18}$

$\therefore x = 4\sqrt[3]{18}$